adjusted Generic Extraction for PCF with TT except for recursion

theories/GenExtract/GenExtractPCF.v
@@ -10,24 +10,52 @@ Module Env.
     | 0 => False
     | S m => option (fin m)
     end.
+
+  Fixpoint fin_to_nat {n:nat} : fin n -> nat :=
+    match n with
+      0 => @False_rect _
+    | S n => fun i => match i with
+                    None => 0
+                  | Some i => S (fin_to_nat i)
+                  end
+    end.
+  
   Fixpoint vec (X:Type) n : Type :=
     match n with
       0 => unit
     | S n => X * vec X n
     end.
-  Fixpoint nthV {X m} : forall (n : fin m) (xs: vec X m)  , X :=
-    match m as m return forall (n : fin m) (xs: vec X m)  , X with
+  
+  Fixpoint nth__V {X m} : forall (n : fin m) (xs: vec X m)  , X :=
+    match m with
     | 0 => @False_rect _
     | S m => fun n =>
               match n with
                 None => fun xs => fst xs
-              | Some n => fun xs => nthV n (snd xs)
+              | Some n => fun xs => nth__V n (snd xs)
               end
     end.
 
+  
+  Fixpoint map__V {X Y} (f: X -> Y) {m}: forall (xs: vec X m), vec Y m :=
+    match m with
+      0 => fun _ => tt
+    | S m => fun xs => (f (fst xs),map__V f (snd xs))
+    end.
+
+  (*
+  Lemma cast_nthV_mapV {n} {X Y} (f : X -> Y) i (vs : vec X n):
+    nth__V i (map__V f vs) = f (nth__V i vs).
+  Proof.
+    induction n;cbn in *. easy.
+    destruct i;cbn in *. all:easy.
+  Qed. *)
+
+  
 End Env.
 Import Env.
 
+(*
 Polymorphic Inductive TT : Type -> Type :=
   TyNat : TT nat
 | TyArr {t1 t2} (tt1 : TT t1) (tt2 : TT t2)
@@ -40,77 +68,210 @@ Existing Instance TyNat.
 Existing Instance TyArr.
   
 
-Hint Mode TT + : typeclass_instances. (* treat argument as input and force evar-freeness*)
+Hint Mode TT + : typeclass_instances. (* treat argument as input and force evar-freeness*) *)
 
 (** Extract only very basic functions, which are more or less PCF with "coq-guarded" recursion *)
 
-Notation anyTT := {t : Type & TT t} (only parsing).
+Record anyTT := {aTy : Type ; aTT :> TT aTy}.
 
-Notation typeContext := (vec anyTT).
-Fixpoint valueContext {n} : forall (Γ : typeContext n) , Type :=
-  match n as n return forall (Γ : typeContext n) , Type with
+Coercion Build_anyTT : TT >-> anyTT.
+Existing Class anyTT.
+Existing Instance Build_anyTT.
+
+
+Fixpoint hvec {X} (F: X -> Type) {n} : forall (Γ : vec X n) , Type :=
+  match n with
     0 => fun _ => unit
-  | S n' => fun Γ => (projT1 (fst Γ) * valueContext (snd Γ))%type
+  | S n' => fun Γ => (F (fst Γ) * hvec F (snd Γ))%type
   end.
-Fixpoint nthC {m} : forall {Γ : typeContext m} (n : fin m) (vs: valueContext Γ) , projT1 (nthV n Γ) :=
-  match m as m' return forall  {Γ : typeContext m'} (n : fin m') (vs: @valueContext m' Γ)  , projT1 (nthV n Γ) with
+
+Fixpoint nth__HV {X} {F} {m} : forall {Γ : vec X m} (n : fin m) (vs: hvec F Γ) , F (nth__V n Γ) :=
+  match m with
   | 0 => fun _ f => False_rect _ f
   | S m => (fun Γ n vs =>
            match n with
            | None => fst vs
-           | Some n => nthC n (snd vs)
+           | Some n => nth__HV n (snd vs)
            end)
   end.
 
-Inductive isPCF : forall n (Γ : typeContext n) (A: anyTT), (valueContext Γ -> projT1 A) -> Type :=
+Notation typeContext := (vec anyTT).
+Notation valueContext := (hvec aTy).
+
+From Undecidability Require Import LNat.
+Local Unset Implicit Arguments.
+
+
+Notation TyNat := (@TyB _ registered_nat_enc).
+
+Inductive isPCF : forall n (Γ : typeContext n) (A: anyTT), (valueContext Γ -> A.(aTy)) -> Type :=
   isPCF_Const n Γ (c:nat) :
-    isPCF n Γ (existT _ _ TyNat) (fun _ => c)
-| isPCF_Rel n Γ x :
-    let A := nthV x Γ in @isPCF n Γ A (nthC x)
-| isPCF_App n Γ t1 t2 tt1 tt2
-            (f:valueContext Γ -> t1 -> t2) (arg: valueContext Γ -> t1):
-    isPCF n Γ (existT _ _ (@TyArr t1 t2 tt1 tt2)) f
-    -> @isPCF n Γ (existT _ _ tt1) arg
-    -> @isPCF n Γ (existT _ _ tt2) (fun ctx => (f ctx) (arg ctx))
-| isPCF_Lambda n Γ t1 t2 tt1 tt2 f:
-    isPCF (S n) (existT _ _ tt1,Γ) (existT _ _ tt2) (fun ctx => f (snd ctx) (fst ctx))
-    -> @isPCF n Γ (existT _ _ (@TyArr t1 t2 tt1 tt2)) f
+    isPCF n Γ TyNat (fun _ => c)
+| isPCF_Rel n Γ x : isPCF n Γ (nth__V x Γ) (nth__HV x)
+| isPCF_App n Γ (A B : anyTT)
+            (f:valueContext Γ -> A.(aTy) -> B.(aTy)) (arg: valueContext Γ -> A.(aTy)):
+    isPCF n Γ (TyArr A B) f
+    -> isPCF n Γ A arg
+    -> isPCF n Γ B (fun ctx => (f ctx) (arg ctx))
+| isPCF_Lambda n (Γ : typeContext n) A B (f:valueContext Γ -> _):
+    isPCF (S n) (A,Γ) B (fun ctx => f (snd ctx) (fst ctx))
+    -> @isPCF n Γ (TyArr A B) f
              
-| isPCF_Case_nat n Γ tt x (f__O : valueContext Γ -> projT1 tt) (f__S: valueContext Γ -> nat -> projT1 tt):
-    @isPCF n Γ (existT _ _ TyNat) x
-    -> @isPCF n Γ tt f__O 
-    -> @isPCF (S n) (existT _ _ TyNat,Γ) tt (fun ctx => f__S (snd ctx) (fst ctx))
-    -> @isPCF n Γ tt (fun ctx => match x ctx return projT1 tt with 0 => f__O ctx | S n => f__S ctx n end)
+| isPCF_Case_nat n Γ A x (f__O : valueContext Γ -> A.(aTy)) (f__S: valueContext Γ -> nat -> A.(aTy)):
+    isPCF n Γ TyNat x
+    -> isPCF n Γ A f__O 
+    -> isPCF n Γ (TyArr TyNat A) f__S (* "inlining" means that we can reuse the Lambda-part of proofs *)
+    -> isPCF n Γ A (fun ctx => match x ctx with 0 => f__O ctx | S n => f__S ctx n end)
              
 | isPCF_Succ n Γ:
-    @isPCF n Γ (existT _ _ (TyArr _ _)) (fun _ => S)
-| isPCF_Fix_unaryNat n Γ t tt f F:
-    (forall (ctx : valueContext Γ) (x:nat), F ctx x = f (x,(F ctx,ctx)))
-    -> isPCF (S (S n)) (existT _ _ TyNat,(existT _ _ (@TyArr nat t _ tt),Γ)) (existT _ _ tt) f
-    -> isPCF n Γ (existT _ _ (@TyArr nat t _ tt)) (fun ctx x => F ctx x).
+    @isPCF n Γ (TyArr _ _) (fun _ => S)
+| isPCF_Fix_unaryNat n Γ (A:anyTT) f (F : valueContext Γ -> nat -> A.(aTy))
+                     (H__Fix : forall (ctx : valueContext Γ) (x:nat), F ctx x = f (x,(F ctx,ctx))) :
+    isPCF (S (S n)) ({|aTT := TyNat|},({|aTT := TyArr TyNat A|},Γ)) A f
+    -> isPCF n Γ {|aTT := TyArr TyNat A|} (fun ctx x => F ctx x).
+
+Arguments isPCF_Const {n Γ} c.
+Arguments isPCF_Rel {n Γ} _.
+Arguments isPCF_App {n Γ A B f arg}.
+Arguments isPCF_Lambda {n Γ A B f}.
+Arguments isPCF_Case_nat {n Γ A x f__O f__S}.
+Arguments isPCF_Succ {n Γ}.
+Arguments isPCF_Fix_unaryNat {n Γ A f F _} _.
+
+Arguments isPCF {_} _ _ _.
 
 (* Missing: Fixes, match nat*)
 
 (*Lemma isPCF_mono : isPCF n Γ tt f *)
 
-Lemma isPCF_plus n Γ: isPCF n Γ (existT _ _ (TyArr _ _)) (fun _ => plus).
+Lemma isPCF_plus n (Γ: typeContext n): isPCF Γ (TyArr _ (TyArr _ _)) (fun _ => plus).
 Proof.
   unfold Init.Nat.add.
-  simple eapply isPCF_Fix_unaryNat with (f:= fun ctx=> fun m => match fst ctx with
-                                                          | 0 => m
-                                                          | S p => S (fst (snd ctx) p m)
-                                                          end).
+  apply @isPCF_Fix_unaryNat with (A := {| aTT := (TyArr TyNat TyNat) |} )
+                                 (f:= fun ctx=> fun m => match fst ctx with
+                                                   | 0 => m
+                                                   | S p => S (fst (snd ctx) p m)
+                                                   end).
   now intros arg [].
-  simple eapply isPCF_Lambda.
-  simple eapply isPCF_Case_nat.
-  -eapply (isPCF_Rel (3+_)) with (x:=Some None).
-  -eapply (isPCF_Rel (3+_)) with (x:=None).
-  -eapply isPCF_App. now econstructor. cbn. 
-   eapply isPCF_App with (f:= fun ctx => fst (snd (snd (snd ctx))) (fst ctx));cbn.
-   2:now eapply (isPCF_Rel (4+_)) with (x:=Some None).
-   eapply isPCF_App with (f:= fun ctx => fst (snd (snd (snd ctx))));cbn.
-   now eapply (isPCF_Rel (4+_)) with (x:=Some (Some (Some None))).
-   now eapply (isPCF_Rel (4+_)) with (x:=None).
+  eapply @isPCF_Lambda with (A := TyNat) (B := TyNat).
+  simple eapply @isPCF_Case_nat.
+  -eapply @isPCF_Rel with (x:=Some None).
+  -eapply @isPCF_Rel with (x:=None).
+  -eapply @isPCF_Lambda with (A := TyNat) (B := TyNat).
+   eapply @isPCF_App with (A := TyNat). now econstructor. cbn. 
+   eapply @isPCF_App with (A := TyNat) (f:= fun ctx => fst (snd (snd (snd ctx))) (fst ctx));cbn.
+   2:now eapply @isPCF_Rel with (x:=Some None).
+   eapply @isPCF_App with (A := TyNat) (f:= fun ctx => fst (snd (snd (snd ctx))));cbn.
+   now eapply @isPCF_Rel with (x:=Some (Some (Some None))).
+   now eapply @isPCF_Rel with (x:=None).
+Defined.
+
+From Undecidability Require Import LNat.
+
+
+Local Notation "↑ env" := (0,map__V S env) (at level 10).
+
+Fixpoint PCFtoL {n} {Γ : typeContext n} {A:anyTT} {f:valueContext Γ -> A.(aTy)} (H : isPCF Γ A f): vec nat n -> term :=
+  match H with
+  | @isPCF_Const n Γ c => fun ren => enc c
+  | @isPCF_Rel n Γ x =>  fun ren => var (nth__V x ren)
+  | @isPCF_App n Γ A B f arg H__f H__arg =>  fun ren => app (PCFtoL H__f ren) (PCFtoL H__arg ren)
+  | @isPCF_Lambda n Γ A B f H__f =>  fun ren => lam (PCFtoL H__f (↑ ren))
+
+  (* TODO: lambda-lift for "lazy" evaluation?*)
+  | @isPCF_Case_nat n Γ A x f__O f__S H__x H__O H__S =>  fun ren => app (app (PCFtoL H__x ren) (PCFtoL H__O ren)) (PCFtoL H__S ren)
+                                                  
+  | @isPCF_Succ n Γ =>  fun ren => ext S
+  | @isPCF_Fix_unaryNat n Γ A f F H__Fix H__F =>  fun ren => rho (lam (lam (PCFtoL H__F (0,(1,map__V S ren)))))
+  end.
+
+Fixpoint vec_to_list {n X} : vec X n -> list X :=
+  match n with
+    0 => fun _ => nil
+  | S n => fun xs => fst xs :: vec_to_list (snd xs)
+  end.
+
+Lemma In_vec_to_list {X n} (x:X) (v:vec X n):
+  In x (vec_to_list v) -> exists i, nth__V i v = x.
+Proof.
+  induction n;cbn in *. easy. intros [ <- | ]. now eexists None.
+  edestruct IHn as [i ?]. eauto. now eexists (Some i).
 Qed.
 
-     
+
+Lemma extensionalMatch_nat {X} (T : X -> Type) n H__O H__S:
+  T (match n with 0 => H__O | S n => H__S n end) = match n with 0 => T H__O | S n => T (H__S n) end.
+Proof.
+  now destruct n.
+Defined.
+
+
+Lemma dualMatch_nat X Y (T : X -> Y -> Type) n H1__O H1__S H2__O H2__S:
+  T (match n with 0 => H1__O | S n => H1__S n end) (match n with 0 => H2__O | S n => H2__S n end) = match n with 0 => T H1__O H2__O | S n => T (H1__S n) (H2__S n) end.
+Proof.
+  now destruct n.
+Defined.
+
+
+Lemma nat_case {X} (T : X -> Type) H__O H__S:
+  T H__O -> (forall n, T (H__S n)) -> forall n, T (match n with 0 => H__O | S n => H__S n end).
+Proof.
+  now intros ? ? [].
+Defined.
+
+
+Lemma isPCP_L_computable {n} {Γ : typeContext n} {A:anyTT} {f:valueContext Γ -> A.(aTy)}
+      (H : isPCF Γ A f) (vs : valueContext Γ) (env__L : vec term n) (ren : vec nat n) :
+  hvec proc env__L ->
+  {v & (LClos.substList (PCFtoL H ren) 0 (vec_to_list env__L) >* v) * computes A.(aTT) (f vs) v}%type.
+Proof.
+  induction H;intros proc__env.
+  1:{(* Const*) do 2 esplit. cbn. rewrite LClos.substList_closed. 1,3:reflexivity. Lproc. }
+  1:{(*Rel*) cbn. rewrite Nat.sub_0_r. do 2 esplit. reflexivity. admit. }
+  1:{(*App*) cbn. edestruct IHisPCF2  with (1:=proc__env) as (v2&R2&IH2). 
+      cbn in IHisPCF1. edestruct IHisPCF1 as (v&R&Hproc&v'&R'&IH1). 1,2:eassumption.
+      eexists;split. 2:easy. rewrite R,R2. easy.
+  }
+  1:{ (*Lambda *) cbn.
+      eexists. split. reflexivity. split. split. 2:easy.
+      { (*PCFtoL is closed *) admit. }
+      intros.
+      edestruct IHisPCF with (vs := (a,vs)) (env__L := (t_a,env__L)) as (v&R&IH).
+      {split;cbn. all:eauto using computesProc. }
+
+      cbn in IH.
+      eexists. split. 
+      rewrite step_Lproc. 2:now eapply computesProc. 2:exact IH.
+      rewrite LClos.subst_substList. eassumption.
+      { hnf. intros ? (i&<-)%In_vec_to_list. now destruct (nth__HV i proc__env). }
+  }
+  1:{ (* Case_nat *) cbn.
+      specialize IHisPCF1 with (vs:=vs) (ren:=ren) (env__L := env__L) (1:=proc__env).
+      specialize IHisPCF2 with (vs:=vs) (ren:=ren) (env__L := env__L) (1:=proc__env).
+      specialize IHisPCF3 with (vs:=vs) (ren:=ren) (env__L := env__L) (1:=proc__env).
+
+      edestruct IHisPCF1 as (_ &R__x &[= -> ]).
+      edestruct IHisPCF2 as (v__O &R__O &IH__O).
+      edestruct IHisPCF3 as (v__S &R__S &IH__S).
+      clear IHisPCF1. clear IHisPCF2. clear IHisPCF3. 
+
+      eexists. split. 2:erewrite dualMatch_nat.
+      { rewrite R__x,R__O,R__S. rewrite nat_enc_correct. 2,3:now eapply computesProc;eassumption.
+       
+        destruct (x vs). reflexivity.
+        hnf in IH__S. 
+
+        set (proc__v:= fst IH__S).
+        set (IH__v:= snd IH__S a _ eq_refl).
+        set (IH := (fst (projT2 IH__v))). subst IH__v. 
+        eapply IH.
+      }
+      destruct (x vs). easy.
+      set (proc__v:= fst IH__S). cbn in IH__S. 
+      set (IH__v:= snd IH__S a _ eq_refl).
+      set (IH := (snd (projT2 IH__v))). subst IH__v.
+      exact IH.
+  }
+  1:{(* Succ *) eexists;split. reflexivity. cbn - [computes]. rewrite LClos.substList_closed. 2:now Lproc. apply extCorrect. }
+  1:{(* Fix_unaryNat *) cbn - [rho]. admit. }
+Admitted.
