theories/GenExtract/GenExtractPCF_noTT.v
@@ -10,11 +10,22 @@ Module Env.
     | 0 => False
     | S m => option (fin m)
     end.
+
+  Fixpoint fin_to_nat {n:nat} : fin n -> nat :=
+    match n with
+      0 => @False_rect _
+    | S n => fun i => match i with
+                    None => 0
+                  | Some i => S (fin_to_nat i)
+                  end
+    end.
+  
   Fixpoint vec (X:Type) n : Type :=
     match n with
       0 => unit
     | S n => X * vec X n
     end.
+  
   Fixpoint nthV {X m} : forall (n : fin m) (xs: vec X m)  , X :=
     match m with
     | 0 => @False_rect _
@@ -25,6 +36,12 @@ Module Env.
               end
     end.
 
+  Fixpoint mapV {X Y} (f: X -> Y) {m}: forall (xs: vec X m), vec Y m :=
+    match m with
+      0 => fun _ => tt
+    | S m => fun xs => (f (fst xs),mapV f (snd xs))
+    end.
+      
 End Env.
 Import Env.
 
@@ -59,7 +76,7 @@ Inductive isPCF : forall n (Γ : typeContext n) (A: Type), (valueContext Γ -> A
     -> @isPCF n Γ A arg
     -> @isPCF n Γ B (fun ctx => (f ctx) (arg ctx))
 | isPCF_Lambda n (Γ : typeContext n) A B (f:valueContext Γ -> _):
-    isPCF (S n) (A,Γ) B(fun ctx => f (snd ctx) (fst ctx))
+    isPCF (S n) (A,Γ) B (fun ctx => f (snd ctx) (fst ctx))
     -> @isPCF n Γ (A -> B) f
              
 | isPCF_Case_nat n Γ A x (f__O : valueContext Γ -> A) (f__S: valueContext Γ -> nat -> A):
@@ -70,33 +87,91 @@ Inductive isPCF : forall n (Γ : typeContext n) (A: Type), (valueContext Γ -> A
              
 | isPCF_Succ n Γ:
     @isPCF n Γ (nat -> nat) (fun _ => S)
-| isPCF_Fix_unaryNat n Γ A f F:
-    (forall (ctx : valueContext Γ) (x:nat), F ctx x = f (x,(F ctx,ctx)))
-    -> isPCF (S (S n)) (nat:Type,(nat -> A,Γ)) A f
+| isPCF_Fix_unaryNat n Γ A f F
+                     (H__Fix : forall (ctx : valueContext Γ) (x:nat), F ctx x = f (x,(F ctx,ctx))) :
+    isPCF (S (S n)) (nat:Type,(nat -> A,Γ)) A f
     -> isPCF n Γ (nat -> A) (fun ctx x => F ctx x).
+
+Arguments isPCF_Const {n Γ} c.
+Arguments isPCF_Rel {n Γ} _.
+Arguments isPCF_App {n Γ A B f arg}.
+Arguments isPCF_Lambda {n Γ A B f}.
+Arguments isPCF_Case_nat {n Γ A x f__O f__S}.
+Arguments isPCF_Succ {n Γ}.
+Arguments isPCF_Fix_unaryNat {n Γ A f F _} _.
+
+Arguments isPCF {_} _ {_} _.
 
 (* Missing: Fixes, match nat*)
 
 (*Lemma isPCF_mono : isPCF n Γ tt f *)
 
-Lemma isPCF_plus n Γ: isPCF n Γ _ (fun _ => plus).
+Lemma isPCF_plus n (Γ: typeContext n): isPCF Γ (fun _ => plus).
 Proof.
   unfold Init.Nat.add.
-  simple eapply isPCF_Fix_unaryNat with (f:= fun ctx=> fun m => match fst ctx with
+  eapply @isPCF_Fix_unaryNat with (f:= fun ctx=> fun m => match fst ctx with
                                                           | 0 => m
                                                           | S p => S (fst (snd ctx) p m)
                                                           end).
   now intros arg [].
   simple eapply isPCF_Lambda.
-  simple eapply isPCF_Case_nat.
-  -eapply (isPCF_Rel (3+_)) with (x:=Some None).
-  -eapply (isPCF_Rel (3+_)) with (x:=None).
+  simple eapply @isPCF_Case_nat.
+  -eapply @isPCF_Rel with (x:=Some None).
+  -eapply @isPCF_Rel with (x:=None).
   -eapply isPCF_App. now econstructor. cbn. 
-   eapply isPCF_App with (f:= fun ctx => fst (snd (snd (snd ctx))) (fst ctx));cbn.
-   2:now eapply (isPCF_Rel (4+_)) with (x:=Some None).
-   eapply isPCF_App with (f:= fun ctx => fst (snd (snd (snd ctx))));cbn.
-   now eapply (isPCF_Rel (4+_)) with (x:=Some (Some (Some None))).
-   now eapply (isPCF_Rel (4+_)) with (x:=None).
+   eapply @isPCF_App with (f:= fun ctx => fst (snd (snd (snd ctx))) (fst ctx));cbn.
+   2:now eapply @isPCF_Rel with (x:=Some None).
+   eapply @isPCF_App with (f:= fun ctx => fst (snd (snd (snd ctx))));cbn.
+   now eapply @isPCF_Rel with (x:=Some (Some (Some None))).
+   now eapply @isPCF_Rel with (x:=None).
+Defined.
+
+From Undecidability Require Import LNat.
+
+
+Local Notation "↑ env" := (0,mapV S env) (at level 10).
+
+Lemma cast_nthV_mapV {n} {X Y} (f : X -> Y) i (vs : vec X n):
+  nthV i (mapV f vs) = f (nthV i vs).
+Proof.
+  induction n;cbn in *. easy.
+  destruct i;cbn in *. all:easy.
 Qed.
 
-     
+Import JMeq EqdepFacts.
+
+(* Maybe rensert TT ? *)
+Definition PCFtoTT : forall {n} {Γ : typeContext n} {A:Type} {f:valueContext Γ -> A} (H : isPCF Γ f),
+    valueContext (mapV TT Γ) -> {tt : TT A & forall R, tt = @TyB A R -> JMeq R registered_nat_enc }.
+Proof.
+  refine (fix PCFtoTT {n} {Γ : typeContext n} {A:Type} {f:valueContext Γ -> A} (H : isPCF Γ f):
+            valueContext (mapV TT Γ) -> {tt : TT A & forall R, tt = @TyB A R -> JMeq R registered_nat_enc } :=
+            match H with
+            | @isPCF_Const n Γ c => fun ren => existT _ (TyB nat) _
+            | @isPCF_Rel n Γ x _ =>  fun ren => existT _ (@eq_rect _ _ id (nthC x ren) _ (cast_nthV_mapV TT x Γ))  _
+            | @isPCF_App n Γ A B f arg H__f H__arg =>
+              fun ren => existT _ _ (match projT1 (PCFtoTT H__f ren)  with @TyArr A' B' tA' tB' => _ | @TyB A' tA' => _ end) (*fun ren => app (PCFtoL H__f ren) (PCFtoL H__arg ren) *)
+            | @isPCF_Lambda n Γ A B f H__f => _
+            | @isPCF_Case_nat n Γ A x f__O f__S H__x H__O H__S => _
+            | @isPCF_Succ n Γ => fun ren => existT _ (TyArr (TyB nat) (TyB nat)) _
+            | @isPCF_Fix_unaryNat n Γ A f F H__Fix H__F => _
+            end).
+  abstract (now intros ? [=]; apply eq_dep_JMeq,eq_sigT_iff_eq_dep).
+  intros ?
+
+Fixpoint PCFtoL {n} {Γ : typeContext n} {A:Type} {f:valueContext Γ -> A} (H : isPCF Γ f): vec nat n -> term :=
+  match H with
+  | @isPCF_Const n Γ c => fun ren => enc c
+  | @isPCF_Rel n Γ x _ =>  fun ren => var (nthV x ren)
+  | @isPCF_App n Γ A B f arg H__f H__arg =>  fun ren => app (PCFtoL H__f ren) (PCFtoL H__arg ren)
+  | @isPCF_Lambda n Γ A B f H__f =>  fun ren => lam (PCFtoL H__f (↑ ren))
+
+  (* TODO: lambda-lift for "lazy" evaluation?*)
+  | @isPCF_Case_nat n Γ A x f__O f__S H__x H__O H__S =>  fun ren => app (app (PCFtoL H__x ren) (PCFtoL H__O ren)) (PCFtoL H__S (↑ ren))
+                                                  
+  | @isPCF_Succ n Γ =>  fun ren => ext S
+  | @isPCF_Fix_unaryNat n Γ A f F H__Fix H__F =>  fun ren => rho (lam (lam (PCFtoL H__F (0,(1,mapV S ren)))))
+  end.
+
+Lemma isPCP_L_computable {n} {Γ : typeContext n} {A:Type} {f:valueContext Γ -> A} (H : isPCF Γ f) ren :
+  computes
